- change the meaning of DeclCtx - more progress on progress lemma

SystemFD/Metatheory/Progress.lean
@@ -31,9 +31,16 @@ inductive Val : Ctx Term -> Term -> Prop where
   | app : t.neutral_form = .some (n, ts)
         -> Γ.is_stable n
         -> Val Γ t
+  | appk : Val Γ (f `@k a)
   | lam :  Val Γ (`λ[a] b)
   | lamt : Val Γ (Λ[A] b)
   | refl : Val Γ (refl! _)
+  | star : Val Γ ★
+  | arr :  Val Γ (A -t> B)
+  | arrk : Val Γ (A -k> B)
+  | all : Val Γ (∀[A]B)
+  | eq : Val Γ (A ~ B)
+
 
 theorem flip_eq : Γ ⊢ (A ~ B) : ★ -> Γ ⊢ (B ~ A) : ★ := by
 intros h; cases h; case _ k AJ BJ => apply Judgment.eq k BJ AJ
@@ -47,6 +54,16 @@ theorem datatype_kind : ⊢ Γ -> Γ d@ x = .datatype t -> Γ ⊢ t : .kind := b
 intros wΓ h;
 sorry
 
+theorem kind_kind : ⊢ Γ -> Γ d@ x = .kind t -> Γ ⊢ t : .kind := by
+intros wΓ h;
+sorry
+
+
+theorem openm_type : ⊢ Γ -> Γ d@ x = .openm t -> Γ ⊢ t : .type := by
+intros wΓ h;
+sorry
+
+
 theorem not_neutral_form_shape : Val Γ t ->
         t.neutral_form = .some (n, ts)
         -> ¬ ((t = `λ[A] b)
@@ -56,8 +73,8 @@ theorem not_neutral_form_shape : Val Γ t ->
             ∨ t = .ite p s b c
             ∨ t = .kind
             ∨ t = .type
-            ∨ t = refl! A
-            ∨ t = sym! η
+            -- ∨ t = refl! A
+            -- ∨ t = sym! η
             ) := by
 intros tnf; induction t;
 any_goals (solve | simp_all)
@@ -82,20 +99,6 @@ theorem invert_all_kind : (Γ ⊢ ∀[ A ] B : w) -> w = ★ := by
 intros eqJ; cases eqJ; simp_all;
 
 
-theorem test : ⊢ Γ -> ¬ Γ.is_stable x -> ¬ (Γ d@ x).get_type = .some (A ~ B) := by sorry
-
-def DeclCtx (Γ : Ctx Term) : Prop := ∀ n, ¬ Γ.is_lam_bound n
-
-theorem invert_appk_val : Γ ⊢ t : (A -k> B)
-                       -> Val Γ t -> t.neutral_form = .none
-                       -> t = Λ[A] t' := by
-intros tJ vt tnotnormal; induction vt;
-case _ => simp_all
-case _ => cases tJ
-case _ => cases tJ
-case _ => cases tJ
-
-
 theorem lamt_typing_unique : Γ ⊢ Λ[A]b : t -> ∃ B', t = ∀[A] B' := by
 intros tJ; cases tJ;
 case _ => simp_all;
@@ -107,6 +110,37 @@ case _ => simp_all;
 theorem refl_typing_unique : Γ ⊢ refl! A : t -> (t = (A ~ A)) := by
 intros tJ; cases tJ;
 case _ => simp_all;
+
+
+theorem test : ⊢ Γ -> ¬ Γ.is_stable x -> ¬ (Γ d@ x).get_type = .some (A ~ B) := by sorry
+
+inductive DeclCtx  : (Γ : Ctx Term) -> Prop where
+|  nil : DeclCtx []
+|  consempty : DeclCtx Γ -> DeclCtx (.empty :: Γ)
+|  conskind : DeclCtx Γ -> DeclCtx (.kind K :: Γ)
+|  consdt : DeclCtx Γ -> DeclCtx (.datatype K :: Γ)
+|  consom : DeclCtx Γ -> DeclCtx (.openm K :: Γ)
+|  consterm : DeclCtx Γ -> DeclCtx (.term A t :: Γ)
+|  consinst : DeclCtx Γ -> DeclCtx (.inst n A :: Γ)
+
+theorem no_lam_bindings : (DeclCtx Γ) -> ∀ x, ¬  (Γ d@ x = .type T) := by
+intro dctx; induction dctx;
+case _ => simp_all;
+case _ ih => intros x; have hh := ih x; sorry;
+case _ => sorry;
+case _ => sorry;
+case _ => sorry;
+case _ => sorry;
+case _ => sorry;
+
+theorem dt_is_dt {Γ : Ctx Term}: Γ d@x = Frame.datatype t -> (Γ d@ x).is_datatype := by
+intros dt; simp_all; unfold Frame.is_datatype; simp;
+
+theorem dt_is_stable {Γ : Ctx Term}{x : Nat}: Γ d@ x = Frame.datatype t -> Frame.is_stable (Γ d@ x) := by
+intros dt; unfold Frame.is_stable; rw [dt];
+
+theorem opent_is_stable {Γ : Ctx Term}: Γ d@x = Frame.opent t -> Frame.is_stable (Γ d@ x) := by
+intros dt; unfold Frame.is_stable; rw [dt];
 
 theorem apptneqrefl : ¬ ((f `@t a) = (refl! A)) := by simp_all
 theorem appneqrefl : ¬ ((f `@ a) = (refl! A)) := by simp_all
@@ -154,11 +188,36 @@ case _ =>
     have reds := Exists.intro w h; simp_all;
 case _ => cases tred; case _ h =>
   cases h;
+  case _ => sorry; -- bogus case
+  case _ => sorry; -- bogus case
+
+case _ => cases tred; case _ h =>
+  cases h;
   case _ => simp_all
   case _ => simp_all
 case _ => cases tred; case _ h =>
   cases h;
   case _ => simp_all
+  case _ => simp_all
+case _ => cases tred; case _ h =>
+  cases h;
+  case _ => simp_all
+  case _ => simp_all
+case _ => cases tred; case _ h =>
+  cases h;
+  case _ => simp_all
+  case _ => simp_all
+case _ => cases tred; case _ h =>
+  cases h;
+  case _ => simp_all
+  case _ => simp_all
+case _ => cases tred; case _ h =>
+  cases h;
+  case _ => simp_all
+  case _ => simp_all
+case _ => cases tred; case _ h =>
+  cases h;
+  case _ => simp_all;
   case _ => simp_all
 case _ => cases tred; case _ h =>
   cases h;
@@ -225,26 +284,29 @@ case _ Γ t n _ _ n_stable =>
       have lem := classification_lemma aj; simp at lem; cases lem;
       case _ h => cases h
       case _ h => cases h; case _ h => cases h.2; simp_all;
-
+case _ => cases ηJ; simp_all; sorry
 case _ => cases ηJ
 case _ => cases ηJ
 case _ => cases ηJ; simp_all
+case _ => cases ηJ
+case _ => cases ηJ
+case _ => cases ηJ
+case _ => cases ηJ
+case _ => cases ηJ
 
 
 @[simp]
 abbrev StepOrVal : (v : JudgmentVariant) -> (Γ : Ctx Term) -> (JudgmentArgs v) -> Prop
-| .prf => λ Γ => λ(t , A) => DeclCtx Γ -> (∃ K, Γ ⊢ K : .kind ∧ Γ ⊢ A : K) -> Val Γ t ∨ ∃ t', Red Γ t t'
+| .prf => λ Γ => λ(t , _) => Val Γ t ∨ ∃ t', Red Γ t t'
 | .wf  => λ _ => λ () => true
 
-
 theorem progress :
-   ⊢ Γ
+   ⊢ Γ -> DeclCtx Γ
   -> Judgment v Γ ix
 --------------------------------------
   -> StepOrVal v Γ ix := by
-intros wΓ j; induction j;
-any_goals (solve | simp at *)
-all_goals (intro dctx h)
+intros wΓ dctx j; induction j;
+any_goals (solve | simp_all)
 case _ Γ A t b _ _ _ _ _ _ _ ih _ =>
   simp_all;
   generalize tl' : [b β[ t ]] = t' at *; symm at tl';
@@ -252,41 +314,33 @@ case _ Γ A t b _ _ _ _ _ _ _ ih _ =>
   have ereds : ∃ t', Red Γ (.letterm A t b) t' := Exists.intro t' reds;
   apply Or.inr ereds;
 
-case _ => cases h; case _ h => cases h.2;
+case _ => simp_all; apply Or.inl Val.star;
 case var Γ x _ _ xTy ih =>
-  simp at ih; have x_no_lam := dctx x;
-  unfold Ctx.is_lam_bound at x_no_lam;
-  unfold Frame.is_lam_bound at x_no_lam;
+  simp at ih;
   unfold Frame.get_type at xTy; simp at xTy;
   split at xTy;
   any_goals (solve | simp_all)
-  case _ x_is_datatype => cases h; case _ w h =>
-    cases h; case _ w h =>
-      injection xTy with xt; subst xt;
-      have lem := classification_lemma h; simp at lem; cases lem;
-      case _ h => subst h; cases w
-      case _ h =>
-        simp_all; have lem := classification_lemma h; simp at lem; cases lem;
-        case _ h => cases h; cases w
-        case _ =>
-             have ttt := datatype_kind wΓ x_is_datatype;
-             have ut := uniqueness_of_types ttt h; subst ut; cases w;
+  case _ f _ x_is_kind =>
+    simp_all; have xK := kind_kind wΓ x_is_kind;
+    subst xTy;
+    sorry
+  case _ f _ x_is_type => exfalso; apply no_lam_bindings dctx x x_is_type;
+  case _ f _ x_is_datatype =>
+      simp_all; have x_is_stable := dt_is_stable x_is_datatype;
+      have hh : (#x).neutral_form = .some (x, []) := Term.var_neutral_form;
+      apply Or.inl;
+      apply Val.app hh x_is_stable;
 
   case _ f t x_is_ctor =>
     have xx : Frame.is_stable (Γ d@ x) := by unfold Frame.is_stable; rw[x_is_ctor];
     have hh : (#x).neutral_form = .some (x, []) := Term.var_neutral_form;
     apply Or.inl (Val.app hh xx)
-  case _ x_is_opent =>
-    injection xTy with teqT; symm at teqT; subst teqT;   -- classification lemma
-    cases h; case _ h =>
-      cases h; case _ t w _ h =>
-      simp_all;
-      have lem := classification_lemma h; simp at lem; cases lem;
-      case _ l h => subst h; cases l
-      case _ l _ =>
-        have ttt := opent_kind wΓ x_is_opent;
-        have ut := uniqueness_of_types ttt h; subst ut; cases l;
 
+  case _ x_is_opent =>
+      have x_is_stable := opent_is_stable x_is_opent;
+      have hh : (#x).neutral_form = .some (x, []) := Term.var_neutral_form;
+      apply Or.inl;
+      apply Val.app hh x_is_stable;
   case _ x_is_openm =>  -- steps inst
     have nf  := @Term.var_neutral_form x; symm at nf;
     have om : (Γ d@ x).is_openm := by unfold Frame.is_openm; rw [x_is_openm];
@@ -305,53 +359,84 @@ case var Γ x _ _ xTy ih =>
     have etl' : ∃ t', Red Γ (#x) t' := Exists.intro ([t.apply_spine []]) (Red.letterm nf x_is_term);
     apply Or.inr etl'
 
-case _ => cases h; case _ h => cases h.2
-case _ => cases h; case _ h => cases h.2; cases h.1;
+case _ => simp_all; apply Or.inl; apply Val.arrk
+case _ => simp_all; apply Or.inl; apply Val.all
+case _ => simp_all; apply Or.inl; apply Val.arr
 
-case _ => cases h; case _ h => cases h.2; cases h.1
-case appk Γ f A B a fJ aJ  fs as =>  -- bogus case
-  cases h; case _ h =>
-    have lem := classification_lemma fJ; simp at lem; cases lem;
-    case _ w h' => have hB := h.2; cases h'; case _ hB' =>
-      have wKind := uniqueness_of_types hB hB'; subst wKind; cases h.1;
-    case _ h => cases h; case _ w h => cases h.2; case _ h => cases h; case _ w h => cases w
+case appk fs as => simp_all;  apply Or.inl; apply Val.appk
 
-case _ => cases h; case _ h => cases h.2; cases h.1
+case _ => simp_all; apply Or.inl; apply Val.eq
 
-case ite Γ p A s _ i _ _ e _ _ _ _ _ _ _ _ tstar _ pJ sJ _ iJ _ eJ =>
-  simp_all; cases h; case _ w h =>
-  have weqstar := uniqueness_of_types tstar h.2; subst weqstar; simp_all;
-  have pJ' := pJ ★ h.1;
-  -- prefix_type_match
-  sorry
+case ite Γ p A s _ i _ _ e _ _ RJ _ vhvp vhvr _ _ tstar _ ps ss _ is _ es =>
+  simp_all; cases ps;
+  case inr h => cases h; case _ p' redp =>
+    cases vhvp; case _ pnf h =>
+    simp_all; have pctor := h.2;
+    have pnp := h.1; symm at pnp;
+    have head_stable := Frame.is_ctor_implies_is_stable pctor;
+    have pnf_val := Val.app pnp head_stable;
+    have pnr := val_no_red pnf_val; simp_all;
+
+  case inl h =>
+    cases h;
+    case _ => cases vhvp; case _ n sp _ _ _  h =>
+      simp_all; cases ss;
+      case inl pnf sv => -- s is a value
+        cases sv;
+        case _ sJ => sorry
+        case _ sJ => sorry
+        case _ sJ => sorry
+        case _ sJ => sorry
+        case _ sJ =>
+          have h := refl_typing_unique sJ;  cases h; case _ => cases vhvr; sorry
+        case _ sJ => sorry
+        case _ sJ => have risStar := invert_arr_kind sJ; subst risStar; cases RJ
+        case _ sJ => sorry
+        case _ sJ => have risStar := invert_all_kind sJ; subst risStar; cases RJ
+        case _ sJ => have risStar := invert_eq_kind sJ; subst risStar; cases RJ
+
+      case _ h =>
+        cases h;
+        case _ w h =>
+          generalize tlp : List.map (Term.ite p · i e) w = tl' at *; symm at tlp;
+          have reds : ∃ t', Red Γ (.ite p s i e) t' := Exists.intro tl' (Red.ite_congr h tlp);
+          apply Or.inr reds
+
+    case _ => cases vhvp; case _ h =>
+      simp at h; have h1 := h.1; have wctor := h.2;  sorry
+    case _ => cases vhvp; simp_all;
+    case _ => cases vhvp; simp_all;
+    case _ => cases vhvp; simp_all;
+    case _ => cases vhvp; simp_all;
+    case _ => cases vhvp; simp_all
+    case _ => cases vhvp; simp_all
+    case _ => cases vhvp; simp_all
+    case _ => cases vhvp; simp_all
 
 case guard => sorry
 
 case _ _ A t _ _ _ _ _ _ _ => apply Or.inl Val.lam
 
 case app Γ f A B a B' fJ aJ _ fs as =>
-  simp_all; cases h; case _ w h =>
-  have lem := classification_lemma fJ; simp at lem; cases lem;
-  case _ h => cases h;
-  case _ h => cases h; case _ w' h' =>
-  have weqstar := invert_arr_kind h'.2; subst weqstar;
-  cases h'.2; cases h'.1;
-  have fs' := @fs ★ (h'.1) h'.2;
-  cases fs';
+  simp_all; cases fs;
   case inl h => -- f is value
     cases h;
     case app n ts n_stable fnf =>
-      have fanf := @Term.neutral_form_app f a n ts fnf;
-      apply Or.inl (Val.app fanf n_stable);
-    case lam  => cases h; case _ a' b l r =>
+       have fanf := @Term.neutral_form_app f a n ts fnf;
+       apply Or.inl (Val.app fanf n_stable);
+    case lam A B =>
       apply Or.inr;
-      have reds : ∃ t', Red Γ ((`λ[a']b) `@ a) t' := Exists.intro [b β[ a ]] (@Red.beta Γ a' b a);
+      have reds : ∃ t', Red Γ ((`λ[A]B) `@ a) t' := Exists.intro [B β[ a ]] (@Red.beta Γ A B a);
       apply reds
-    case lamt =>
-      cases h; case _ A' b l r =>
-        have xx := lamt_typing_unique fJ; cases xx; case _ w h => cases h;
-    case refl =>
-        have xx := refl_typing_unique fJ; cases xx
+    case lamt  => have xx := lamt_typing_unique fJ; cases xx; case _ w h => cases h;
+    case refl => have xx := refl_typing_unique fJ; cases xx
+    case _ => sorry
+    case _ => have fJ' := Judgment.ax wΓ; have u := uniqueness_of_types fJ fJ'; cases u;
+    case _ => cases fJ
+    case _ => cases fJ;
+    case _ => cases fJ
+    case _ => cases fJ
+
   case inr h => cases h; case _ w h => -- f steps
     generalize tlp : List.map (· `@ a) w = tl' at *; symm at tlp;
     have reds : ∃ t', Red Γ (f `@ a) t' := Exists.intro tl' (Red.app_congr h tlp);
@@ -360,46 +445,40 @@ case app Γ f A B a B' fJ aJ _ fs as =>
 case _ _ A t _ _ _ _ _ _ _ => apply Or.inl Val.lamt
 
 case appt Γ f _ _ a _ fJ aJ _ fs as =>
-  simp_all; cases h; case _ w h =>
-  have lem := classification_lemma fJ; simp at lem; cases lem;
-  case _ h => cases h
-  case _ h => cases h; case _ w' h' =>
-    have weqstar := invert_all_kind h'.2; subst weqstar;
-    cases h'.2; cases h'.1; have fs' := @fs ★ h'.1 h'.2; cases fs';
-    case inr h => cases h; case _ w h =>
+  simp_all; cases fs;
+  case inr h => cases h; case _ w h =>
       apply Or.inr;
       generalize tlp : List.map (· `@t a) w = tl' at *; symm at tlp;
       have reds : ∃ t', Red Γ (f `@t a) t' := Exists.intro tl' (Red.appt_congr h tlp);
-      apply reds
-    case inl h =>
+      apply reds;
+  case inl h =>
     cases h;
     case app n ts n_stable fnf =>
       have fanf := @Term.neutral_form_appt f a n ts fnf
       apply Or.inl;
       apply (Val.app fanf n_stable);
-    case lam => cases h; case _ a' b l r =>
-        have xx := lam_typing_unique fJ; cases xx; simp_all;
+    case lam => have xx := lam_typing_unique fJ; cases xx; simp_all;
     case lamt a' b =>
       apply Or.inr;
       have reds : ∃ t', Red Γ ((Λ[a']b) `@t a) t' := Exists.intro [b β[ a ]] (@Red.betat Γ a' b a);
       apply reds
-    case refl =>
-        have xx := refl_typing_unique fJ; cases xx
+    case refl => have xx := refl_typing_unique fJ; cases xx
+    case _ => cases fJ; case _ h =>  sorry
+    case _ => have fJ' := Judgment.ax wΓ; have xx := uniqueness_of_types fJ fJ'; cases xx
+    case _ => cases fJ
+    case _ => cases fJ
+    case _ => cases fJ
+    case _ => cases fJ
 
 case _ Γ t A η B tJ ηJ ts cs =>
-  simp_all; cases h; case _ w h =>
-  have lem := classification_lemma ηJ; simp at lem; cases lem; cases h;
-  case _ eqJ _ h => cases eqJ
-  case _ h => cases h; case _ w h =>
-    have weqstar := invert_eq_kind h.2; subst weqstar;
-    have cs' := @cs ★ h.1 h.2; cases cs';
-    case _ h =>
+  simp_all; cases cs;
+  case _ h =>
       have ηreflp := @refl_is_val Γ η A B dctx ηJ h;
       have ηrefl := ηreflp.1;
       subst ηrefl; apply Or.inr;
       have reds : ∃ t', Red Γ (t ▹ refl! A) t' := Exists.intro [t] Red.cast;
-      apply reds;
-    case _ h => cases h; case _ w h =>
+      apply reds
+  case _ h => cases h; case _ w h =>
       apply Or.inr
       generalize tlp : List.map (t ▹ ·) w = tl' at *; symm at tlp;
       have reds : ∃ t', Red Γ (t ▹ η) t' := Exists.intro tl' (Red.cast_congr h tlp);
@@ -407,11 +486,7 @@ case _ Γ t A η B tJ ηJ ts cs =>
 
 case _ => apply Or.inl Val.refl
 case sym Γ η A B ηJ ηs =>
-  cases h; case _ w h =>
-  have h2 := invert_eq_kind h.2; subst h2;
-  have h2 := flip_eq h.2;
-  simp at ηs; have ηs' := @ηs wΓ dctx ★ h.1 h2;
-  cases ηs';
+  cases ηs wΓ dctx;
   case _ h =>
     have x := refl_is_val dctx ηJ h;
     have xeqrefl := x.left;
@@ -425,98 +500,128 @@ case sym Γ η A B ηJ ηs =>
     generalize tlp : List.map (sym! ·) w = tl' at *; symm at tlp;
     have reds : ∃ t', Red Γ (sym! η) t' := Exists.intro tl' (Red.sym_congr h tlp);
     apply reds;
-case seq η1J η2J η1s η2s =>
-  simp_all; cases h; case _ w h =>
-    have weqstr := invert_eq_kind h.2; subst weqstr;
-    have η1s' := η1s ★ h.1;
-    sorry
-case appc Γ A K1 K2 B η1 C D η2 aK bK η1J cJ dJ η2J _ _ η1s _ _ η2s  =>
-  -- check if η1 reduces or η2 reduces if both are values then reduce to refl
-  simp_all; cases h; case _ w h =>
-  have weqstr := invert_eq_kind h.2; subst weqstr;
-  have lemA := classification_lemma aK; simp at lemA;
-  cases lemA;
-  case _ wA arrk1k2 =>
-    have η1s' := η1s ★ h.1 (Judgment.eq arrk1k2 aK bK);
-    cases η1s';
-    case _ vη1 =>
-      have η1refl := refl_is_val dctx η1J vη1;
-      have aeqB := η1refl.2; have η1rfl := η1refl.1;
-      -- subst aeqB; subst η1rfl; simp at *;
-      have lemC := classification_lemma cJ; simp at lemC; cases lemC;
-      case _ k1ki =>
 
-        -- have eqCDstar := @invert_eq_kind Γ C D sorry;
-        -- have η2s' := η2s ★ (Judgment.eq k1ki cJ dJ);
-        sorry
-      case _ hB =>
-        cases hB;
-        case _ k1ki =>
-          have eqCDstar := @invert_eq_kind Γ C D ★;
-          -- have η2s' := η2s ★ (Judgment.eq k1ki cJ dJ);
-          sorry
-        case _ h => cases h; case _ w h => sorry
-
-    case _ h =>
-      apply Or.inr; cases h; case _ w tl =>
-      generalize tlp : List.map (· `@c η2) w = tl' at *; symm at tlp;
-      have reds : ∃ t', Red Γ (η1 `@c η2) t' := Exists.intro tl' (Red.appc_congr1 tl tlp);
-      apply reds
-
-  case _ wB hB => cases hB; case _ w h => cases h.2; case _ h => cases h.1
-
-case arrowc => -- check if η1 reduces or η2 reduces if both are values then reduce to refl
-  cases h; case _ w h =>
-  cases h; case _ w h =>
-    have keqstr := invert_eq_kind h; subst keqstr;
-    have lem := classification_lemma h; simp at lem; cases lem;
-    case _ h => sorry
-    case _ h => sorry
-
-case fst =>
-  sorry
-case snd η _ _ _ _ _ _ _ _ _ ηs =>
-  simp_all; cases h; case _ w h =>
-  have weqstr := invert_eq_kind h.2; subst weqstr;
-  have ηs' := ηs ★ h.1;
-  sorry
-case _ K A B t allAJ allBJ _ _ _ ts =>
-  -- cases h; case _ w h =>
-  -- have weqstr := invert_eq_kind h.2; subst weqstr;
-  -- simp at ts;
-  -- cases h.2; case _ h =>
-  --   have ts' := ts sorry (Judgment.wfkidctx ★ (Judgment.ax sorry) ; sorry
-  cases h; case _ h =>
-  cases h.2; cases h.1;
-  have lem := classification_lemma h.2; simp at lem; cases lem;
-  case _ allAJ' allBJ' _ _ =>
-   have keq := uniqueness_of_types allAJ' allAJ; subst keq;
-   sorry
-  case _ h => cases h; case _ allAJ' allBJ' _ _ _ =>
-   cases h.2; cases h.1; have keq := uniqueness_of_types allAJ' allAJ; subst keq;
-   sorry
-
-case _ Γ η1 K A B C D η2 _ _ η1J CKJ _ η2J _ _ η1s _ _ η2s =>
-  simp_all; cases h; case _ w h =>
-  have lem := classification_lemma η2J; simp at lem; cases lem;
-  case _ h => cases h;
-  case _ h => cases h; case _ w' h' =>
-  have weqstar := invert_eq_kind h'.2; subst weqstar;
-  cases h'.2; cases h'.1; have η2s' := @η2s ★ h'.1 h'.2;
-  cases η2s';
+case seq Γ η1 A B η2 C η1J η2J η1s η2s =>
+  simp_all; cases η2s;
   case _ h =>
     have η2refp := refl_is_val dctx η2J h;
-    have η2refl := η2refp.1; -- subst ηrefl;
-    have lem := classification_lemma η1J; simp at lem; cases lem;
-    case _ h => cases h;
-    case _ h => cases h; case _ K' _ CKJ' _ _ w' h' =>
-    have kk' := uniqueness_of_types CKJ CKJ'; subst kk';
-    have weqstar := invert_eq_kind h'.2; subst weqstar;
-    cases h'.2; cases h'.1; have η1s' := @η1s ★ h'.1 h'.2;
-    cases η1s';
+    have η2refl := η2refp.1; cases η1s;
     case _ h =>
       have η1refp := refl_is_val dctx η1J h;
-      have η1refl := η1refp.1; -- subst ηrefl;
+      have η1refl := η1refp.1; have aeqB := η1refp.2; have BeqC := η2refp.2
+      subst η1refl; subst η2refl;
+      apply Or.inr; subst aeqB;
+      have reds : ∃ t', Red Γ ((refl! A) `; (refl! A)) t' := Exists.intro [refl! A] Red.seq;
+      apply reds
+    case _ h => cases h; case _ w h =>
+      apply Or.inr;
+      generalize tlp : List.map (· `; η2) w = tl' at *; symm at tlp;
+      have reds : ∃ t', Red Γ (η1 `; η2) t' := Exists.intro tl' (Red.seq_congr1 h tlp);
+      apply reds
+  case _ h => cases h; case _ w h =>
+    apply Or.inr;
+    generalize tlp : List.map (η1 `; ·) w = tl' at *; symm at tlp;
+    have reds : ∃ t', Red Γ (η1 `; η2) t' := Exists.intro tl' (Red.seq_congr2 h tlp);
+    apply reds
+
+case appc Γ A K1 K2 B η1 C D η2 aK bK η1J cJ dJ η2J _ _ η1s _ _ η2s  =>
+  -- check if η1 reduces or η2 reduces if both are values then reduce to refl
+  simp_all; cases η2s;
+  case _ h =>
+    have η2refp := refl_is_val dctx η2J h;
+    have η2refl := η2refp.1; cases η1s;
+    case _ h =>
+      have η1refp := refl_is_val dctx η1J h;
+      have η1refl := η1refp.1; -- have aeqB := η1refp.2; have BeqC := η2refp.2
+      subst η1refl; subst η2refl;
+      apply Or.inr;
+      have reds : ∃ t', Red Γ ((refl! A) `@c (refl! C)) t' := Exists.intro [refl! (A `@k C)] Red.appc;
+      apply reds
+    case _ h => cases h; case _ w h =>
+      apply Or.inr;
+      generalize tlp : List.map (· `@c η2) w = tl' at *; symm at tlp;
+      have reds : ∃ t', Red Γ (η1 `@c η2) t' := Exists.intro tl' (Red.appc_congr1 h tlp);
+      apply reds
+  case _ h => cases h; case _ w h =>
+    apply Or.inr;
+    generalize tlp : List.map (η1 `@c ·) w = tl' at *; symm at tlp;
+    have reds : ∃ t', Red Γ (η1 `@c η2) t' := Exists.intro tl' (Red.appc_congr2 h tlp);
+    apply reds
+
+case arrowc Γ A B η1 C D η2 _ _ η1J _ _ η2J _ _ η1s _ _ η2s =>
+  simp_all; cases η2s (Judgment.wfempty wΓ) (DeclCtx.consempty dctx);
+  case _ h =>
+    have dctx' : DeclCtx (Frame.empty :: Γ) := DeclCtx.consempty dctx;
+    have η2refp := refl_is_val dctx' η2J h;
+    have η2refl := η2refp.1; cases η1s;
+    case _ h =>
+      have η1refp := refl_is_val dctx η1J h;
+      have η1refl := η1refp.1;
+      subst η1refl; subst η2refl;
+      apply Or.inr;
+      have reds : ∃ t', Red Γ (refl!(A) -c> refl! C) t' := Exists.intro [(refl! (A -t> C))] Red.arrowc;
+      apply reds
+    case _ h => cases h; case _ w h =>
+      apply Or.inr;
+      generalize tlp : List.map (· -c> η2) w = tl' at *; symm at tlp;
+      have reds : ∃ t', Red Γ (η1 -c> η2) t' := Exists.intro tl' (Red.arrowc_congr1 h tlp);
+      apply reds
+  case _ h => cases h; case _ w h =>
+    apply Or.inr;
+    generalize tlp : List.map (η1 -c> ·) w = tl' at *; symm at tlp;
+    have reds : ∃ t', Red Γ (η1 -c> η2) t' := Exists.intro tl' (Red.arrowc_congr2 h tlp);
+    apply reds
+
+case fst Γ A _ _ _ η C _ _ _ ηJ _ _ ηs =>
+  simp_all; cases ηs;
+  case inl h =>
+    have ηrp := refl_is_val dctx ηJ h; have ηrfl := ηrp.1; subst ηrfl;
+    apply Or.inr;
+    have reds : ∃ t', Red Γ ((refl! (A `@k C)).!1) t' := Exists.intro [refl! A] Red.fst;
+    apply reds;
+  case inr h => cases h; case _ w h =>
+    apply Or.inr;
+    generalize tlp : List.map (·.!1) w = tl' at *; symm at tlp;
+    have reds : ∃ t', Red Γ (η.!1) t' := Exists.intro tl' (Red.fst_congr h tlp);
+    apply reds
+
+case snd Γ _ C _ η A _ _ _ _ ηJ _ _ _ ηs =>
+  simp_all; cases ηs;
+  case inl h =>
+    have ηrp := refl_is_val dctx ηJ h; have ηrfl := ηrp.1; subst ηrfl;
+    apply Or.inr;
+    have reds : ∃ t', Red Γ ((refl! (A `@k C)).!2) t' := Exists.intro [refl! C] Red.snd;
+    apply reds;
+  case inr h => cases h; case _ w h =>
+    apply Or.inr;
+    generalize tlp : List.map (·.!2) w = tl' at *; symm at tlp;
+    have reds : ∃ t', Red Γ (η.!2) t' := Exists.intro tl' (Red.snd_congr h tlp);
+    apply reds
+
+case _ Γ K A B η allAJ allBJ ηJ _ _ ts =>
+  cases allAJ; case _ kkind _ =>
+  have ts := ts (Judgment.wfkind kkind wΓ) (DeclCtx.conskind dctx);
+  cases ts;
+  case inr h => cases h; case _ w h =>
+    simp_all;
+    apply Or.inr;
+    generalize tlp : List.map (∀c[K]·) w = tl' at *; symm at tlp;
+    have reds : ∃ t', Red Γ (∀c[K] η) t' := Exists.intro tl' (Red.allc_congr h tlp);
+    apply reds
+  case inl h =>
+    have ηrp := refl_is_val (DeclCtx.conskind dctx) ηJ h; have ηrfl := ηrp.1; subst ηrfl;
+    apply Or.inr;
+    have reds : ∃ t', Red Γ ((∀c[K] refl! A)) t' := Exists.intro [refl! (∀[K]A)] Red.allc;
+    apply reds;
+
+case _ Γ η1 K A B C D η2 _ _ η1J CKJ _ η2J _ _ η1s _ _ η2s =>
+  simp_all; cases η2s;
+  case _ h =>
+    have η2refp := refl_is_val dctx η2J h;
+    have η2refl := η2refp.1; cases η1s;
+    case _ h =>
+      have η1refp := refl_is_val dctx η1J h;
+      have η1refl := η1refp.1;
       subst η1refl; subst η2refl;
       apply Or.inr;
       have reds : ∃ t', Red Γ (refl!(∀[K] A) `@c[refl! C]) t' := Exists.intro [refl! (A β[ C ])] Red.apptc;
